src/Syntax.v
@@ -169,8 +169,7 @@ Record System oifc :=
     sys_merqs: list IdxT;
     sys_merss: list IdxT;
     sys_msg_inds_valid: NoDup (sys_minds ++ sys_merqs ++ sys_merss);
-    sys_oss_inits: OStates oifc;
-    sys_orqs_inits: ORqs Msg
+    sys_oss_inits: OStates oifc
   }.
 
 Lemma obj_same_id_in_system_same:
@@ -190,9 +189,6 @@ Ltac inds_valid_tac :=
 
 Global Instance System_OStates_HasInit {oifc}: HasInit (System oifc) (OStates oifc) :=
   {| initsOf := @sys_oss_inits _ |}.
-
-Global Instance System_ORqs_HasInit {oifc}: HasInit (System oifc) (ORqs Msg) :=
-  {| initsOf := @sys_orqs_inits _ |}.
 
 Close Scope string.
 Close Scope list.
